shift-reset/core/ident.v
@@ -1,0 +1,6 @@
+From Stdlib Require Import String.
+
+Record ident : Type := Ident { ident_car : string }.
+
+Definition ident_eq_dec : forall (x1 x2 : ident), {x1 = x2} + {x1 <> x2}.
+Proof. decide equality; auto using string_dec. Defined.
