shift-reset/core/var.v
@@ -1,6 +1,0 @@
-From Stdlib Require Import String.
-
-Record var : Type := Var { var_car : string }.
-
-Definition var_eq_dec : forall (x1 x2 : var), {x1 = x2} + {x1 <> x2}.
-Proof. decide equality; auto using string_dec. Defined.
